code/hash/Hacl.Hash.SHA2.fst
@@ -1,14 +1,120 @@
 module Hacl.Hash.SHA2
 
+module ST = FStar.HyperStack.ST
+module HS = FStar.HyperStack
+
 open Hacl.Hash.Definitions
 open Spec.Hash.Definitions
 
+open Lib.MultiBuffer
+open Lib.NTuple
+
 include Hacl.Hash.Core.SHA2
 
-friend Hacl.Hash.MD
+// To prove we are properly defining init
+friend Spec.Agile.Hash
+// To prove we are properly defining update_last
+friend Spec.Hash.Incremental
+// To know the definition of init
+friend Spec.SHA2
 
-let update_multi_224 =
-  Hacl.Hash.MD.mk_update_multi SHA2_224 update_224
+#set-options "--fuel 0 --ifuel 0 --z3rlimit 100"
+
+let mb_init_is_init (#a: sha2_alg) (h: HS.mem) (st: state (| a, () |) ): Lemma
+  (requires (LowStar.Buffer.as_seq h st == Hacl.Spec.SHA2.Vec.(init a M32)))
+  (ensures (as_seq h st == Spec.Agile.Hash.init a))
+=
+  let st1 = as_seq h st in
+  let st1_raw = LowStar.Buffer.as_seq h st in
+  let spec = Spec.Agile.Hash.init a in
+  let spec_vec = Hacl.Spec.SHA2.Vec.(init a M32) in
+  assert (st1_raw `Seq.equal` spec_vec);
+  let t = Spec.Hash.Definitions.word_t a in
+  let h0 = Hacl.Spec.SHA2.h0 a in
+  let lemma_i (i: nat { i < 8 }): Lemma
+    (Seq.index st1 i == Seq.index spec i)
+  =
+    calc (== ) {
+      Seq.index st1 i;
+    (==) { }
+      Seq.index (Lib.IntVector.vec_v #t #1 (Seq.index spec_vec i)) 0;
+    (==) { (* otherwise the pattern on createi doesn't trigger *) }
+      Seq.index (Lib.IntVector.vec_v #t #1 (Lib.Sequence.index spec_vec i)) 0;
+    (==) { }
+      Seq.index (Lib.IntVector.vec_v #t #1 Hacl.Spec.SHA2.Vec.(load_element a M32
+        (Seq.index h0 i))) 0;
+    (==) { }
+      Seq.index (Lib.IntVector.vec_v #t #1 Lib.IntVector.(
+        vec_load (Seq.index h0 i) 1)) 0;
+    (==) { }
+      Seq.index h0 i;
+    };
+    ()
+  in
+  FStar.Classical.forall_intro lemma_i;
+  assert (st1 `Seq.equal` spec)
+
+let init_224 st =
+  Hacl.SHA2.Scalar32.init #SHA2_224 st;
+  let h1 = ST.get () in
+  mb_init_is_init h1 st
+
+let init_256 st =
+  Hacl.SHA2.Scalar32.init #SHA2_256 st;
+  let h1 = ST.get () in
+  mb_init_is_init h1 st
+
+let init_384 st =
+  Hacl.SHA2.Scalar32.init #SHA2_384 st;
+  let h1 = ST.get () in
+  mb_init_is_init h1 st
+
+let init_512 st =
+  Hacl.SHA2.Scalar32.init #SHA2_512 st;
+  let h1 = ST.get () in
+  mb_init_is_init h1 st
+
+let alloca_224 () =
+  let h0 = ST.get () in
+  let st = Hacl.Impl.SHA2.Generic.alloc SHA2_224 Hacl.Spec.SHA2.Vec.M32 in
+  Hacl.Impl.SHA2.Generic.init st;
+  let h1 = ST.get () in
+  mb_init_is_init #SHA2_224 h1 st;
+  LowStar.Buffer.(modifies_only_not_unused_in loc_none h0 h1);
+  st
+
+let alloca_256 () =
+  let h0 = ST.get () in
+  let st = Hacl.Impl.SHA2.Generic.alloc SHA2_256 Hacl.Spec.SHA2.Vec.M32 in
+  Hacl.Impl.SHA2.Generic.init st;
+  let h1 = ST.get () in
+  mb_init_is_init #SHA2_256 h1 st;
+  LowStar.Buffer.(modifies_only_not_unused_in loc_none h0 h1);
+  st
+
+let alloca_384 () =
+  let h0 = ST.get () in
+  let st = Hacl.Impl.SHA2.Generic.alloc SHA2_384 Hacl.Spec.SHA2.Vec.M32 in
+  Hacl.Impl.SHA2.Generic.init st;
+  let h1 = ST.get () in
+  mb_init_is_init #SHA2_384 h1 st;
+  LowStar.Buffer.(modifies_only_not_unused_in loc_none h0 h1);
+  st
+
+let alloca_512 () =
+  let h0 = ST.get () in
+  let st = Hacl.Impl.SHA2.Generic.alloc SHA2_512 Hacl.Spec.SHA2.Vec.M32 in
+  Hacl.Impl.SHA2.Generic.init st;
+  let h1 = ST.get () in
+  mb_init_is_init #SHA2_512 h1 st;
+  LowStar.Buffer.(modifies_only_not_unused_in loc_none h0 h1);
+  st
+
+let update_multi_224 st () blocks n_blocks =
+  let blocks1 = ntup1 blocks in
+  Hacl.SHA2.Scalar32.sha224_update_nblocks (n_blocks `FStar.UInt32.mul` block_len SHA2_224) blocks1 st;
+  admit ()
+
 let update_multi_256 =
   Hacl.Hash.MD.mk_update_multi SHA2_256 update_256
 let update_multi_384 =
