code/hash/Hacl.Hash.SHA2.fsti
@@ -3,18 +3,58 @@ module Hacl.Hash.SHA2
 open Hacl.Hash.Definitions
 open Spec.Hash.Definitions
 
-include Hacl.Hash.Core.SHA2
+inline_for_extraction noextract
+val init_224: init_st (|SHA2_224, ()|)
+inline_for_extraction noextract
+val init_256: init_st (|SHA2_256, ()|)
+inline_for_extraction noextract
+val init_384: init_st (|SHA2_384, ()|)
+inline_for_extraction noextract
+val init_512: init_st (|SHA2_512, ()|)
 
+inline_for_extraction noextract
+val alloca_224: alloca_st (|SHA2_224, ()|)
+inline_for_extraction noextract
+val alloca_256: alloca_st (|SHA2_256, ()|)
+inline_for_extraction noextract
+val alloca_384: alloca_st (|SHA2_384, ()|)
+inline_for_extraction noextract
+val alloca_512: alloca_st (|SHA2_512, ()|)
+
+inline_for_extraction noextract
 val update_multi_224: update_multi_st (|SHA2_224, ()|)
+inline_for_extraction noextract
 val update_multi_256: update_multi_st (|SHA2_256, ()|)
+inline_for_extraction noextract
 val update_multi_384: update_multi_st (|SHA2_384, ()|)
+inline_for_extraction noextract
 val update_multi_512: update_multi_st (|SHA2_512, ()|)
 
+inline_for_extraction noextract
 val update_last_224: update_last_st (|SHA2_224, ()|)
+inline_for_extraction noextract
 val update_last_256: update_last_st (|SHA2_256, ()|)
+inline_for_extraction noextract
 val update_last_384: update_last_st (|SHA2_384, ()|)
+inline_for_extraction noextract
 val update_last_512: update_last_st (|SHA2_512, ()|)
 
+inline_for_extraction noextract
+val finish_224: finish_st (|SHA2_224, ()|)
+inline_for_extraction noextract
+val finish_256: finish_st (|SHA2_256, ()|)
+inline_for_extraction noextract
+val finish_384: finish_st (|SHA2_384, ()|)
+inline_for_extraction noextract
+val finish_512: finish_st (|SHA2_512, ()|)
+
+// Leaving these for backwards-compat, for now. TODO: investigate and see if we
+// can:
+// - mark these as inline_for_extraction
+// - rename the new-ish hash functions in Hacl_Streaming_SHA2
+// - rename Hacl_Streaming_SHA2 into Hacl_SHA2
+// - use krml's rename-prefix to obtain exactly the same function names (with
+//   identical argument orders)
 val hash_224: hash_st SHA2_224
 val hash_256: hash_st SHA2_256
 val hash_384: hash_st SHA2_384
